03: add inductions

03-untyped/03Untyped/Basic.lean
@@ -1,1 +1,68 @@
-def hello := "world"
+import Mathlib.Tactic.Basic
+
+
+namespace Section3
+
+inductive Lang
+| zero
+| True
+| False
+| succ (exp : Lang)
+| pred (exp : Lang)
+| iszero (exp : Lang)
+| If (cond exp₁ exp₂ : Lang)
+
+def size : Lang → Nat
+| .zero => 1
+| .True => 1
+| .False => 1
+| .succ exp => 1 + size exp
+| .pred exp => 1 + size exp
+| .iszero exp => 1 + size exp
+| .If cond exp₁ exp₂ => 1 + size cond + size exp₁ + size exp₂
+
+
+def depth : Lang → Nat
+| .zero => 1
+| .True => 1
+| .False => 1
+| .succ exp => 1 + depth exp
+| .pred exp => 1 + depth exp
+| .iszero exp => 1 + depth exp
+| .If cond exp₁ exp₂ => 1 + max (max (depth cond) (depth exp₁)) (depth exp₂)
+
+lemma induction_size_specified (P : Lang → Prop) :
+  ∀ gen_sz, (∀ (s : Lang), (∀ r, size r < size s → P r) → P s) → ∀ s, size s < gen_sz  → P s := by
+    intro gen_sz ind s hlt
+    induction gen_sz generalizing s
+    { simp [*] at hlt }
+    rename_i n hn
+    by_cases size s = n
+    { grind }
+    grind
+
+theorem induction_size (P : Lang → Prop) :
+  (∀ (s : Lang), (∀ r, size r < size s → P r) → P s) → ∀ s, P s := by
+    intro ind s
+    exact induction_size_specified P (size s + 1) ind s (by simp)
+
+
+lemma induction_depth_specified (P : Lang → Prop) :
+  ∀ gen_sz, (∀ (s : Lang), (∀ r, depth r < depth s → P r) → P s) →
+  ∀ s, depth s < gen_sz  → P s := by
+    intro gen_sz ind s hlt
+    induction gen_sz generalizing s
+    { simp [*] at hlt }
+    rename_i n hn
+    by_cases depth s = n
+    { grind }
+    grind
+
+theorem induction_depth (P : Lang → Prop) :
+  (∀ (s : Lang), (∀ r, depth r < depth s → P r) → P s) → ∀ s, P s := by
+    intro ind s
+    exact induction_depth_specified P (depth s + 1) ind s (by simp)
+
+#check Lang.recOn
+
+end Section3
